Rename two utils

io/RILang.fst
@@ -28,6 +28,13 @@ instance rilang_resexn (pi:monitorable_prop) t1 {| d1:rilang t1 pi |} : rilang (
 
 type rilang_dm (pi:monitorable_prop) (a:Type) = c:(IO.Sig.iio a){pi_as_hist pi `Hist.hist_ord` IIO.dm_iio_theta c} 
 
+let as_rilang_dm (w:IIO.dm_iio 'a (pi_as_hist 'p)) : rilang_dm 'p 'a = w
+
+let as_iio_dm (w:rilang_dm 'p 'a) : IIO.dm_iio 'a (pi_as_hist 'p) = 
+  let tree : IO.Sig.iio 'a = w in
+  assert (pi_as_hist 'p `Hist.hist_ord` IIO.dm_iio_theta tree);
+  tree
+
 type rilang_arrow_typ (t1 t2:Type) pi = t1 -> rilang_dm pi t2
 
 instance rilang_arrow (#pi1 #pi2 pi:monitorable_prop) #t1 (d1:rilang t1 pi1) #t2 (d2:rilang t2 pi2) : rilang (rilang_arrow_typ t1 t2 pi) pi =
